src/tls/ConnInvariant.fst
@@ -22,10 +22,10 @@ module SeqP = FStar.SeqProperties
 ////////////////////////////////////////////////////////////////////////////////
 let epoch_regions_exist (s:hs) (h0:HST.mem) =
   let epochs = logT s h0 in 
-  Map.contains (HST.HS.h h0) (HS.region s)
+  Map.contains (HST.HS?.h h0) (HS?.region s)
   /\ (forall (k:nat{k < Seq.length epochs}).{:pattern (Seq.index epochs k)}
       let wr = writer_epoch (Seq.index epochs k) in
-      Map.contains (HST.HS.h h0) (StAE.region wr))
+      Map.contains (HST.HS?.h h0) (StAE.region wr))
 
 #set-options "--initial_fuel 0 --max_fuel 0 --initial_ifuel 0 --max_ifuel 0"
 val frame_epoch_writer: s:hs -> h0:HST.mem -> h1:HST.mem -> 
@@ -34,14 +34,14 @@ val frame_epoch_writer: s:hs -> h0:HST.mem -> h1:HST.mem ->
 		     SeqP.indexable epochs j
 		   /\ epoch_regions_exist s h0 
 		   /\ (let e_j = Seq.index epochs j in
-		      HH.modifies_one (StAE.region (writer_epoch e_j)) (HST.HS.h h0) (HST.HS.h h1))))
+		      HH.modifies_one (StAE.region (writer_epoch e_j)) (HST.HS?.h h0) (HST.HS?.h h1))))
 	(ensures (let epochs0 = logT s h0 in 
 		  let epochs1 = logT s h1 in 
 		  let j = iT s Writer h0 in 
 		  epochs0 == epochs1
 		  /\(forall (k:nat{k < Seq.length epochs0 /\ j<>k}). 
 		      let wr = writer_epoch (Seq.index epochs0 k) in
-		      HH.equal_on (Set.singleton (StAE.region wr)) (HST.HS.h h0) (HST.HS.h h1))))
+		      HH.equal_on (Set.singleton (StAE.region wr)) (HST.HS?.h h0) (HST.HS?.h h1))))
 
 let frame_epoch_writer s h0 h1 = 
   let epochs = logT s h0 in 
@@ -51,7 +51,7 @@ let frame_epoch_writer s h0 h1 =
   let wj = writer_epoch e_j in
   let aux : (k:nat{k < Seq.length epochs /\ j<>k}) -> Lemma 
     (let wr = writer_epoch (Seq.index epochs k) in
-     HH.equal_on (Set.singleton (StAE.region wr)) (HST.HS.h h0) (HST.HS.h h1)) =
+     HH.equal_on (Set.singleton (StAE.region wr)) (HST.HS?.h h0) (HST.HS?.h h1)) =
      fun k -> let wk = writer_epoch (Seq.index epochs k) in
 	   reveal_epochs_inv'();
 	   assert (HH.disjoint (StAE.region wk) (StAE.region wj)) in
@@ -80,11 +80,11 @@ type i_conn (i:id) = r_conn (nonce_of_id i)
       live in distinct regions. 
   -------------------------------------------------------------------------------- *)
 let pairwise_disjoint (m:MM.map' random r_conn) = 
-    forall r1 r2.{:pattern (is_Some (MM.sel m r1));
-		      (is_Some (MM.sel m r2))}
-	r1<>r2 /\ is_Some (MM.sel m r1) /\ is_Some (MM.sel m r2)
-	     ==> HH.disjoint (Some.v (MM.sel m r1)).region  
-		             (Some.v (MM.sel m r2)).region
+    forall r1 r2.{:pattern (Some? (MM.sel m r1));
+		      (Some? (MM.sel m r2))}
+	r1<>r2 /\ Some? (MM.sel m r1) /\ Some? (MM.sel m r2)
+	     ==> HH.disjoint (Some?.v (MM.sel m r1)).region  
+		             (Some?.v (MM.sel m r2)).region
 
 type conn_tab_t = MM.t tls_tables_region random r_conn pairwise_disjoint
 
@@ -115,7 +115,7 @@ let registered (i:id{StAE.is_stream i}) (w:StreamAE.writer i) (c:connection) (h:
   (exists e. (epochs c h) `SeqP.contains` e  /\               //one of c's epochs, e
       (let i' = Epochs.epoch_id e in   //has an id corresponding to i
         i=i' /\ StAE.stream_state #i e.w == w))               //and holds w as as its writer
-  /\ MonSeq.i_contains (MkEpochs.es c.hs.log) h                         //technical: the heap contains c's handshake log
+  /\ MonSeq.i_contains (MkEpochs?.es c.hs.log) h                         //technical: the heap contains c's handshake log
 	
 //The main invariant, relating an ms_tab and a conn_tab at index i, in state h
 let ms_conn_inv (ms:ms_t)
@@ -126,15 +126,15 @@ let ms_conn_inv (ms:ms_t)
      (match MM.sel ms i with 
       | None -> True
       | Some w ->
-        let log_as_hsref = MR.as_hsref (StreamAE.ilog (StreamAE.State.log w)) in
+        let log_as_hsref = MR.as_hsref (StreamAE.ilog (StreamAE.State?.log w)) in
 	//technical: for framing; need to know that the writer's region exists
-	Map.contains (HST.HS.h h) (StreamAE.State.region w) /\  
+	Map.contains (HST.HS?.h h) (StreamAE.State?.region w) /\  
 	//technical: for framing; need to know that when idealized, the log also exists 
-	(authId i ==> HH.contains_ref (HST.MkRef.ref log_as_hsref) (HST.HS.h h)) /\
+	(authId i ==> HH.contains_ref (HST.MkRef?.ref log_as_hsref) (HST.HS?.h h)) /\
 	//main application invariant:
-	(MR.m_sel h (StreamAE.ilog (StreamAE.State.log w)) == Seq.createEmpty  \/   //the writer is either still unused; or
+	(MR.m_sel h (StreamAE.ilog (StreamAE.State?.log w)) == Seq.createEmpty  \/   //the writer is either still unused; or
 	             (let copt = MM.sel conn (nonce_of_id i) in
-  		      is_Some copt /\ registered i w (Some.v copt) h)))            //it's been registered with the connection associated with its nonce
+  		      Some? copt /\ registered i w (Some?.v copt) h)))            //it's been registered with the connection associated with its nonce
 
 //The main invariant, for all AE.ids
 let ms_conn_invariant (ms:ms_t)
@@ -145,9 +145,9 @@ let ms_conn_invariant (ms:ms_t)
 //A technical condition for framing: 
 //    Every handshake region exists in the current heap
 let handshake_regions_exists (conn:c_t) (h:HH.t) = 
-  forall n.{:pattern (is_Some (MM.sel conn n))}
-      is_Some (MM.sel conn n) 
-       ==> (let hs_rgn = HS.region (C.hs (Some.v (MM.sel conn n))) in 
+  forall n.{:pattern (Some? (MM.sel conn n))}
+      Some? (MM.sel conn n) 
+       ==> (let hs_rgn = HS?.region (C.hs (Some?.v (MM.sel conn n))) in 
  	    Map.contains h hs_rgn /\
 	    HH.disjoint hs_rgn tls_tables_region)
 
@@ -155,10 +155,10 @@ let handshake_regions_exists (conn:c_t) (h:HH.t) =
 let mc_inv (h:HST.mem) =
     let conn_tab_as_hsref = MR.as_hsref conn_tab in
     let ms_tab_as_hsref = MR.as_hsref MS.ms_tab in
-    ~ (HH.as_ref (HST.MkRef.ref conn_tab_as_hsref)===HH.as_ref (HST.MkRef.ref ms_tab_as_hsref))   //Technical:the conn_tab and ms_tab are not aliased
-    /\ HH.contains_ref (HST.MkRef.ref conn_tab_as_hsref) (HST.HS.h h)                                //Technical:the heap contains the ms_tab
-    /\ HH.contains_ref (HST.MkRef.ref ms_tab_as_hsref) (HST.HS.h h)                               //Technical:the heap contains the conn_tab
-    /\ handshake_regions_exists (MR.m_sel h conn_tab) (HST.HS.h h)                       //Technical:every logged connection's handshake exists
+    ~ (HH.as_ref (HST.MkRef?.ref conn_tab_as_hsref)===HH.as_ref (HST.MkRef?.ref ms_tab_as_hsref))   //Technical:the conn_tab and ms_tab are not aliased
+    /\ HH.contains_ref (HST.MkRef?.ref conn_tab_as_hsref) (HST.HS?.h h)                                //Technical:the heap contains the ms_tab
+    /\ HH.contains_ref (HST.MkRef?.ref ms_tab_as_hsref) (HST.HS?.h h)                               //Technical:the heap contains the conn_tab
+    /\ handshake_regions_exists (MR.m_sel h conn_tab) (HST.HS?.h h)                       //Technical:every logged connection's handshake exists
     /\ ms_conn_invariant (MR.m_sel h MS.ms_tab) (MR.m_sel h conn_tab) h       //Main joint stateful invariant
 
 (*** PROVING THE STABILITY OF mc_inv ***)
@@ -182,26 +182,26 @@ val ms_derive_is_ok: h0:HST.mem -> h1:HST.mem -> i:AE.id -> w:MS.writer i
 		 let new_ms = MR.m_sel h1 MS.ms_tab in
 		 let ms_tab_as_hsref = MR.as_hsref MS.ms_tab in
 		 mc_inv h0 /\ //we're initially in the invariant
-		 Map.contains (HST.HS.h h1) (StreamAE.State.region w)  /\ //the writer we're adding w is in an existing region
-		 is_epoch_rgn (StreamAE.State.region w) /\     //that it is an epoch region
-		 is_epoch_rgn (HH.parent (StreamAE.State.region w)) /\ //and it's parent is as well (needed for the ms_tab invariant)
-		 HH.modifies (Set.singleton tls_tables_region) (HST.HS.h h0) (HST.HS.h h1) /\ //we just changed the tls_tables_region
-		 HH.modifies_rref tls_tables_region !{HH.as_ref (HST.MkRef.ref ms_tab_as_hsref)} (HST.HS.h h0) (HST.HS.h h1) /\ //and within it, at most the ms_tab
+		 Map.contains (HST.HS?.h h1) (StreamAE.State?.region w)  /\ //the writer we're adding w is in an existing region
+		 is_epoch_rgn (StreamAE.State?.region w) /\     //that it is an epoch region
+		 is_epoch_rgn (HH.parent (StreamAE.State?.region w)) /\ //and it's parent is as well (needed for the ms_tab invariant)
+		 HH.modifies (Set.singleton tls_tables_region) (HST.HS?.h h0) (HST.HS?.h h1) /\ //we just changed the tls_tables_region
+		 HH.modifies_rref tls_tables_region !{HH.as_ref (HST.MkRef?.ref ms_tab_as_hsref)} (HST.HS?.h h0) (HST.HS?.h h1) /\ //and within it, at most the ms_tab
 		 (old_ms == new_ms //either ms_tab didn't change at all  (because we found w in the table already)
 		  \/ (MM.sel old_ms i == None /\ //or, we had to generate a fresh writer w
 		     new_ms == MM.upd old_ms i w /\ //and we just added w to the table
 	   	     (TLSInfo.authId i ==>  //and if we're idealizing i
-		         (let log_as_hsref = MR.as_hsref (StreamAE.ilog (StreamAE.State.log w)) in
-		          HH.contains_ref (HST.MkRef.ref log_as_hsref) (HST.HS.h h1) /\  //the log exists in h1
-			  MR.m_sel h1 (AE.ilog (StreamAE.State.log w)) == Seq.createEmpty))))))       //and w is as yet unused
+		         (let log_as_hsref = MR.as_hsref (StreamAE.ilog (StreamAE.State?.log w)) in
+		          HH.contains_ref (HST.MkRef?.ref log_as_hsref) (HST.HS?.h h1) /\  //the log exists in h1
+			  MR.m_sel h1 (AE.ilog (StreamAE.State?.log w)) == Seq.createEmpty))))))       //and w is as yet unused
 	 (ensures (mc_inv h1))
 val invertOption : a:Type -> Lemma 
   (requires True)
-  (ensures (forall (x:option a). is_None x \/ is_Some x))
+  (ensures (forall (x:option a). None? x \/ Some? x))
   [SMTPatT (option a)]
 let invertOption a = ()  
 	 
-#reset-options "--initial_fuel 0 --max_fuel 0 --initial_ifuel 0 --max_ifuel 0 --z3timeout 100"	 
+#reset-options "--initial_fuel 0 --max_fuel 0 --initial_ifuel 0 --max_ifuel 0 --z3rlimit 100"	 
 let ms_derive_is_ok h0 h1 i w = 
   let aux :  j:id -> Lemma (let new_ms = MR.m_sel h1 MS.ms_tab in
   			  let new_conn = MR.m_sel h1 conn_tab in
@@ -235,7 +235,7 @@ let try_ms_derive (epoch_region:rgn) (i:AE.id)
     MR.m_recall conn_tab;
     MR.m_recall MS.ms_tab;
     let w = MasterSecret.derive epoch_region i in
-    MR.m_recall (AE.ilog (StreamAE.State.log w));
+    MR.m_recall (AE.ilog (StreamAE.State?.log w));
     let h1 = ST.get () in
     ms_derive_is_ok h0 h1 i w;
     w
@@ -258,7 +258,7 @@ let writer_region_within_connection
     (n:random) (c:r_conn n)
     (i:AE.id {nonce_of_id i = n}) (w:AE.writer i) (h:HST.mem)
     : Lemma (requires (registered i w c h))
-	    (ensures (HH.includes (C.region c) (StreamAE.State.region w)))
+	    (ensures (HH.includes (C.region c) (StreamAE.State?.region w)))
     = reveal_epoch_region_inv_all ()
 
 (* Case 2:
@@ -268,29 +268,29 @@ let writer_region_within_connection
       -- so, we're in the "not yet used" case ... so, the epoch's writer is in its initial state and we can return it (our goal is to return a fresh epoch)
 *)
 val register_writer_in_epoch_ok: h0:HST.mem -> h1:HST.mem -> i:AE.id{authId i}
-		-> c:r_conn (nonce_of_id i) -> e:epoch (HS.region c.hs) (nonce_of_id i)
+		-> c:r_conn (nonce_of_id i) -> e:epoch (HS?.region c.hs) (nonce_of_id i)
   -> Lemma (requires
             (let ctab = MR.m_sel h0 conn_tab in
 	     let mstab = MR.m_sel h0 MS.ms_tab in
 	     let old_hs_log = epochs c h0 in
      	     let new_hs_log = epochs c h1 in
-	     let rgn = HS.region c.hs in
+	     let rgn = HS?.region c.hs in
 	     let _ = reveal_epoch_region_inv_all () in
 	     mc_inv h0 /\ //we're initially in the invariant
-	     MonSeq.i_contains (MkEpochs.es c.hs.log) h0 /\
-	     MonSeq.i_contains (MkEpochs.es c.hs.log) h1 /\
+	     MonSeq.i_contains (MkEpochs?.es c.hs.log) h0 /\
+	     MonSeq.i_contains (MkEpochs?.es c.hs.log) h1 /\
 	     i = Epochs.epoch_id e /\ //the epoch has id i
-	     (let w = StAE.stream_state #i (Epoch.w e) in //the epoch writer
-	      let es_log_as_hsref = MR.as_hsref (MkEpochs.es c.hs.log) in
+	     (let w = StAE.stream_state #i (Epoch?.w e) in //the epoch writer
+	      let es_log_as_hsref = MR.as_hsref (MkEpochs?.es c.hs.log) in
 	      let epochs = epochs c h0 in
-              N.registered (nonce_of_id i) (HH.parent (StreamAE.State.region w)) /\  //the writer's parent region is registered in the nonce table
-	      HH.disjoint (HH.parent (StreamAE.State.region w)) tls_region /\          //technical: ... needed just for well-formedness of the rest of the formula
-	      MR.witnessed (MR.rid_exists (StreamAE.State.region w)) /\                //technical: ... needed just for well-formedness of the rest of the formula
+              N.registered (nonce_of_id i) (HH.parent (StreamAE.State?.region w)) /\  //the writer's parent region is registered in the nonce table
+	      HH.disjoint (HH.parent (StreamAE.State?.region w)) tls_region /\          //technical: ... needed just for well-formedness of the rest of the formula
+	      MR.witnessed (MR.rid_exists (StreamAE.State?.region w)) /\                //technical: ... needed just for well-formedness of the rest of the formula
 	      (forall e. epochs `SeqP.contains` e ==> Epochs.epoch_id e <> i) /\            //i is fresh for c
  	      MM.sel mstab i == Some w /\ //we found the writer in the ms_tab
 	      MM.sel ctab (nonce_of_id i) == Some c /\ //we found the connection in the conn_table
-      	      HH.modifies_one (HS.region c.hs) (HST.HS.h h0) (HST.HS.h h1) /\ //we just modified this connection's handshake region
-	      HH.modifies_rref (HS.region c.hs) !{HH.as_ref (HST.MkRef.ref es_log_as_hsref)} (HST.HS.h h0) (HST.HS.h h1) /\ //and within it, just the epochs log
+      	      HH.modifies_one (HS?.region c.hs) (HST.HS?.h h0) (HST.HS?.h h1) /\ //we just modified this connection's handshake region
+	      HH.modifies_rref (HS?.region c.hs) !{HH.as_ref (HST.MkRef?.ref es_log_as_hsref)} (HST.HS?.h h0) (HST.HS?.h h1) /\ //and within it, just the epochs log
 	      new_hs_log == SeqProperties.snoc old_hs_log e))) //and we modified it by adding this epoch to it
 	  (ensures mc_inv h1) //we're back in the invariant
 let register_writer_in_epoch_ok h0 h1 i c e =
@@ -307,22 +307,22 @@ let register_writer_in_epoch_ok h0 h1 i c e =
       let old_conn = MR.m_sel h0 conn_tab in
       let new_conn = MR.m_sel h1 conn_tab in
       let old_hs_log = epochs c h0 in
-      let wi = StAE.stream_state #i (Epoch.w e) in //the epoch writer
+      let wi = StAE.stream_state #i (Epoch?.w e) in //the epoch writer
       let nonce = nonce_of_id i in
       SeqP.contains_intro (SeqP.snoc old_hs_log e) (Seq.length old_hs_log) e;
       SeqP.contains_snoc old_hs_log e; //this lemma shows that everything that was registered to c remains registered to it
       assert (old_ms == new_ms);
       assert (old_conn == new_conn);
-      cut (is_Some (MM.sel old_conn nonce)); //this cut is useful for triggering the pairwise_disjointness quantifier
+      cut (Some? (MM.sel old_conn nonce)); //this cut is useful for triggering the pairwise_disjointness quantifier
       if (authId j && StAE.is_stream j)
       then match MM.sel new_ms j with
            | None -> () //nothing allocated at id j yet; easy
            | Some wj ->
-      	     let log_ref = StreamAE.ilog (StreamAE.State.log wj) in
+      	     let log_ref = StreamAE.ilog (StreamAE.State?.log wj) in
 	     let log_ref_as_hsref = MR.as_hsref log_ref in
-      	     assert (Map.contains (HST.HS.h h1) (StreamAE.State.region wj)); //its region exists; from the 1st technical clause in ms_conn_inv
-      	     assert (HH.contains_ref (HST.MkRef.ref log_ref_as_hsref) (HST.HS.h h1));    //its log exists; from the 2nd technical clause in ms_conn_inv
-	     assert (is_epoch_rgn (StreamAE.State.region wj));    //from the separation clause in ms_con_inv
+      	     assert (Map.contains (HST.HS?.h h1) (StreamAE.State?.region wj)); //its region exists; from the 1st technical clause in ms_conn_inv
+      	     assert (HH.contains_ref (HST.MkRef?.ref log_ref_as_hsref) (HST.HS?.h h1));    //its log exists; from the 2nd technical clause in ms_conn_inv
+	     assert (is_epoch_rgn (StreamAE.State?.region wj));    //from the separation clause in ms_con_inv
       	     let log0 = MR.m_sel h0 log_ref in
       	     let log1 = MR.m_sel h1 log_ref in
       	     assert (log0 == log1); //the properties in the three asserts above are needed to show that j's log didn't change just by registering i
@@ -347,14 +347,14 @@ let register_writer_in_epoch_ok h0 h1 i c e =
 *)
 val mutate_registered_writer_ok : h0:HST.mem -> h1:HST.mem -> i:AE.id{authId i} -> w:MS.writer i -> c:r_conn (nonce_of_id i) -> Lemma
     (requires (mc_inv h0 /\                                       //initially in the invariant
-	       HH.modifies_one (StreamAE.State.region w) (HST.HS.h h0) (HST.HS.h h1) /\ //we modified at most the writer's region
+	       HH.modifies_one (StreamAE.State?.region w) (HST.HS?.h h0) (HST.HS?.h h1) /\ //we modified at most the writer's region
 	       registered i w c h0 /\                             //the writer is registered in c
 	       MM.sel (MR.m_sel h0 MS.ms_tab) i == Some w   /\     //the writer is logged in the ms_tab
 	       MM.sel (MR.m_sel h0 conn_tab) (nonce_of_id i) == Some c /\ //the connection is logged in the conn_table
-	       (let ilog_log_as_hsref = MR.as_hsref (StreamAE.ilog (StreamAE.State.log w)) in
-	        HH.contains_ref (HST.MkRef.ref ilog_log_as_hsref) (HST.HS.h h1)))) //We say that we changed the w.region; but that doesn't necessarily mean that its log remains
+	       (let ilog_log_as_hsref = MR.as_hsref (StreamAE.ilog (StreamAE.State?.log w)) in
+	        HH.contains_ref (HST.MkRef?.ref ilog_log_as_hsref) (HST.HS?.h h1)))) //We say that we changed the w.region; but that doesn't necessarily mean that its log remains
     (ensures (mc_inv h1))
-#set-options "--initial_fuel 0 --max_fuel 0 --initial_ifuel 1 --max_ifuel 1 --z3timeout 100"
+#set-options "--initial_fuel 0 --max_fuel 0 --initial_ifuel 1 --max_ifuel 1 --z3rlimit 100"
 let mutate_registered_writer_ok h0 h1 i w c = (* () *)
 (* a slightly more detailed proof: *)
     let new_ms = MR.m_sel h1 MS.ms_tab in
@@ -379,15 +379,15 @@ let mutate_registered_writer_ok h0 h1 i w c = (* () *)
 (* An auxiliary formula, needed as a pre-condition to add a c to conn_tab *)
 #reset-options "--initial_fuel 0 --max_fuel 0 --initial_ifuel 0 --max_ifuel 0"
 let conn_hs_region_exists (c:connection) (h:HST.mem) =
-   let hs_rgn = HS.region c.hs in
-   Map.contains (HST.HS.h h) hs_rgn /\
+   let hs_rgn = HS?.region c.hs in
+   Map.contains (HST.HS?.h h) hs_rgn /\
    HH.disjoint hs_rgn tls_tables_region
 
 val add_connection_ok: h0:HST.mem -> h1:HST.mem -> i:id -> c:i_conn i -> Lemma
   (requires (let conn_tab_as_hsref = MR.as_hsref conn_tab in
              mc_inv h0 /\ //we're initially in the invariant
-	     HH.modifies (Set.singleton tls_tables_region) (HST.HS.h h0) (HST.HS.h h1) /\  //only modified some table
-	     HH.modifies_rref tls_tables_region !{HH.as_ref (HST.MkRef.ref conn_tab_as_hsref)} (HST.HS.h h0) (HST.HS.h h1) /\ //in fact, only conn_tab
+	     HH.modifies (Set.singleton tls_tables_region) (HST.HS?.h h0) (HST.HS?.h h1) /\  //only modified some table
+	     HH.modifies_rref tls_tables_region !{HH.as_ref (HST.MkRef?.ref conn_tab_as_hsref)} (HST.HS?.h h0) (HST.HS?.h h1) /\ //in fact, only conn_tab
 	     conn_hs_region_exists c h0 /\ //we need to know that c is well-formed
 	     (let old_conn = MR.m_sel h0 conn_tab in
     	      let new_conn = MR.m_sel h1 conn_tab in
@@ -395,10 +395,10 @@ val add_connection_ok: h0:HST.mem -> h1:HST.mem -> i:id -> c:i_conn i -> Lemma
 	      MM.sel old_conn nonce == None /\        //c wasn't in the table initially
 	      new_conn == MM.upd old_conn nonce c))) //and the conn_tab changed just by adding c
   (ensures (mc_inv h1))
-#reset-options "--initial_fuel 0 --max_fuel 0 --initial_ifuel 1 --max_ifuel 1 --z3timeout 100" //NS: this one seems to require an inversion somewhere, but not sure exactly where
+#reset-options "--initial_fuel 0 --max_fuel 0 --initial_ifuel 1 --max_ifuel 1 --z3rlimit 100" //NS: this one seems to require an inversion somewhere, but not sure exactly where
 let add_connection_ok h0 h1 i c =
     cut (let conn_tab_as_hsref = MR.as_hsref conn_tab in
-         HH.contains_ref (HST.MkRef.ref conn_tab_as_hsref) (HST.HS.h h1));
+         HH.contains_ref (HST.MkRef?.ref conn_tab_as_hsref) (HST.HS?.h h1));
     let old_ms = MR.m_sel h0 MS.ms_tab in
     let new_ms = MR.m_sel h1 MS.ms_tab in
     let old_conn = MR.m_sel h0 conn_tab in
@@ -414,4 +414,4 @@ let add_connection_ok h0 h1 i c =
                                      | None -> True
                                      | Some c'' -> c' == c'')) in
     FStar.Classical.forall_intro hs_region_exists;
-    cut (handshake_regions_exists new_conn (HST.HS.h h1))
+    cut (handshake_regions_exists new_conn (HST.HS?.h h1))
