src/tls/HandshakeLog.fst
@@ -45,15 +45,15 @@ let getLogVersion hsl =
 (*   let next = update_hash h eb b in *)
 
 (*
- * AR: changing logref from rref to HS.ref, with region captured in the refinement.
+ * AR: changing logref from rref to HS?.ref, with region captured in the refinement.
  *)
 noeq type log =
   | LOG: #region:rid -> 
-         logref:ref (|
+         logref:ref (
               pv: option protocolVersion
             & (hsl:hs_log{validLog hsl})
             &   b: bytes {getLogVersion hsl = pv /\ handshakeMessagesBytes pv (reveal_hs_log hsl) = b}
-         |){logref.id = region} -> log 
+         ){logref.id = region} -> log 
 
 val create: #reg:rid -> ST log
   (requires (fun h -> True))
@@ -134,7 +134,7 @@ let projectLog_CH (l:hs_log{validLog_CH l}) : logInfo_CH =
     })
 
 val getHash_CH : l:log -> h:CoreCrypto.hash_alg -> 
-  ST (| li:logInfo{is_LogInfo_CH li} & hash:bytes{length hash = CoreCrypto.hashSize h} |)
+  ST ( li:logInfo{LogInfo_CH? li} & hash:bytes{length hash = CoreCrypto.hashSize h} )
     (requires (fun h0 ->
       let lref = l.logref in
       let (| _, hsl, _ |) = sel h0 lref in validLog_CH hsl))
