src/tls/LHAEPlain.fst
@@ -16,7 +16,7 @@ open Range
 // We define payloads and additional data from those of StatefulPlain,
 // adding an 8-byte sequence number to its additional data.
 
-type id = i:id { is_ID12 i }
+type id = i:id { ID12? i }
 
 type seqn = n:nat{repr_bytes n <= 8}
 let ad_Length i = 8 + StatefulPlain.ad_Length i
