src/tls/Nonce.fst
@@ -80,7 +80,7 @@ val mkHelloRandom: cs:role -> r:ex_rid -> ST random
   (ensures (fun h0 n h1 ->
     let nonce_rid_table_as_hsref = MR.as_hsref nonce_rid_table in
     HS.modifies (Set.singleton tls_tables_region) h0 h1 /\ //modifies at most the tables region
-    HS.modifies_ref tls_tables_region !{ HH.as_ref (HS.MkRef.ref nonce_rid_table_as_hsref) } h0 h1 /\ //and within it, at most the nonce_rid_table
+    HS.modifies_ref tls_tables_region !{ HH.as_ref (HS.MkRef?.ref nonce_rid_table_as_hsref) } h0 h1 /\ //and within it, at most the nonce_rid_table
     (ideal ==> fresh n h0  /\        //if we're ideal then the nonce is fresh
     	       registered n r /\     //the nonce n is associated with r
     	       role_nonce cs n r))) //and the triple are associated as well, for ever more
@@ -105,7 +105,7 @@ let lookup role n = MM.lookup nonce_rid_table n
 (* Would be nice to make this a local let in new_region.
    Except, implicit argument inference for testify_forall fails *)
 private let nonce_rids_exists (m:MM.map' random n_rid) = 
-    forall (n:random{is_Some (MM.sel m n)}). MR.witnessed (MR.rid_exists (Some.v (MM.sel m n)))
+    forall (n:random{Some? (MM.sel m n)}). MR.witnessed (MR.rid_exists (Some?.v (MM.sel m n)))
 
 (* 
    A convenient wrapper around FStar.ST.new_region, 
