src/tls/Record.fst
@@ -64,23 +64,20 @@ let parseHeader (h5:header) =
           then Error(AD_illegal_parameter, perror __SOURCE_FILE__ __LINE__ "Wrong fragment length")
           else correct(ct,pv,len)
 
-(* TODO, possibly a parameter from dispatch *)
-assume val is_Null: id -> Tot bool
-
 // hopefully we only care about the writer, not the cn state
 // the postcondition is of the form
 //   authId i ==> f is added to the writer log
 let recordPacketOut (i:StatefulLHAE.id) (wr:StatefulLHAE.writer i) (pv: protocolVersion) f =
     let ct, rg = Content.ct_rg i f in
     let payload =
-      if is_Null i
+      if PlaintextID? i
       then Content.repr i f
       else
         let ad = StatefulPlain.makeAD i ct in
         let f = StatefulPlain.assert_is_plain i ad rg f in
         StatefulLHAE.encrypt #i wr ad rg f
     in
-    makePacket ct (is_Null i) pv payload
+    makePacket ct (PlaintextID? i) pv payload
 
 
 (*** networking (floating) ***)
